exercise5.v
@@ -75,7 +75,7 @@ End Ex1.
 ** Exercise 2:
 
 - Improve on exercise 1 by adding
-  to the [expr] data type a constructor for multiplication and
+  to the [expr] inductive type a constructor for multiplication and
   the simplification rules #$$x * 0 = 0$$# and #$$0 * x = 0$$#
 
 #<div>#
@@ -156,7 +156,7 @@ End Ex2.
 ** Exercise 3:
 
 - Improve on exercise 2 by adding
-  to the [expr] data type a constructor for One and
+  to the [expr] data type a constructor for [One] and
   the simplification rules #$$x * 1 = x$$# and #$$1 * x = x$$#
 
 #<div>#
@@ -236,17 +236,11 @@ Qed.
 
 End Ex3.
 
-
-
 (*
 #</div>#
 
 #</div>#
 ----------------------------------------------------------
-#<div class="slide vfill">#
-
-** To sum up
-
-#</div>#
-----------------------------------------------------------
 *)
+(** When you are done, click the Download link at the top of the page
+    and send us your homework by email: Assia.Mahboubi@inria.fr *)
